\documentclass[12pt, a4paper]{article}
\usepackage[left=1cm, right=1cm, top=1cm, bottom=1.5cm, bindingoffset=0cm]{geometry}
\usepackage{breqn}

\newcommand {\partt} {\frac{\partial}{\partial t}}
\newcommand{\Uxs}[1]{ \frac{f(x)\cdot{#1}^{\alpha-1}}{\Gamma(\alpha)}}
\newcommand {\dt} {\Delta t}
\newcommand {\dx} {\Delta x}

\begin{document}
	\begin{dmath}
	Q1(x,t;s) + {}_{s}D_{t}^{\alpha} V(x,t) + [U(x;s) + V(x,t)]\cdot [ Q2(x,t;s) +  Q3(x,t;s) +  {}_{s}J^{1-\alpha}_{t}V_{x}(x,t)]=a \cdot (U_{xxx}(x;s) + V_{xxx}(x,t))
	\end{dmath}
	
	\begin{equation}
	V(x,t) \bigg{|}_{t=0} = 0, V_{x}(x,t) \bigg{|}_{x=0}=0, V_{x}(x,t) \bigg{|}_{x=1}=0, V_{xx}(x,t) \bigg{|}_{x=1}=0
	\end{equation}

	\begin{equation}
	f(x) = x^{2}(1-x)
	\end{equation}

	\begin{equation}
	U(x;s) = \frac{s^{\alpha-1} \cdot f(x)}{\Gamma(\alpha)}
	\end{equation}

	\begin{equation}
	Q1(x,t;s) = \left(\frac{1}{s} - \frac{1}{t}\right) \frac{\sin(\pi \alpha)}{\pi} \frac{s^{\alpha}}{(t-s)^{\alpha}} f(x)
	\end{equation}

	\begin{equation}
	Q2(x,t;s) =  f^{'}(x) \frac{\sin(\pi \alpha)}{\pi} \frac{1}{\alpha} \frac{s^{\alpha}}{t^{\alpha}} {}_{2}F_{1}\left(\alpha, \alpha, \alpha+1, \frac{s}{t}\right)
	\end{equation}
	
	\begin{equation}
	Q3(x,t;s) = f^{'}(x) \frac{\sin(\pi \alpha)}{\pi} \frac{s^{\alpha - 1}}{(t-s)^{\alpha-1}} \frac{1}{1-\alpha}
	\end{equation}
	
	\begin{equation}
	{}_{2}F_{1}(a,b;c;z) = 1+ \sum_{k = 1}^{\infty} \prod_{l=0}^{k-1} \left[ \frac{(a + l)(b + l)}{(1 + l)(c + l)} \right] z^{k}
	\end{equation}

\noindent\rule{\linewidth}{0.4pt}
	\begin{equation}
	t_{0} = 0, t_{1} = s, t_{2} = s + \Delta t, \dots, t_{n} = s + (n - 1)\Delta t, t_{n+1} = s + n\Delta t
	\end{equation}
	
	\begin{equation}
	x_{i} = i \Delta x
	\end{equation}
	
	\begin{equation}
	V_{0} = V_{1}, V_{N} = V_{N-1} = V_{N-2}
	\end{equation}

\noindent\rule{\linewidth}{0.4pt}
	\begin{dmath}
	{}_{s}D_{t}^{\alpha} V(x_{i},t) = {}_{t_{1}}D_{t_{n+1}}^{\alpha} V(x_{i},t)
	= \dt^{-\alpha} \sum_{j = 0}^{\left[ \frac{t_{n+1} - t_{1}}{\dt}\right]} (-1)^{j} \binom{\alpha}{j} V(x_{i}, t_{n+1} - t_{j})
	= \dt^{-\alpha} \sum_{j = 0}^{\left[ \frac{s + n \dt - s}{\dt}\right]} (-1)^{j} \binom{\alpha}{j} V(x_{i}, t_{n-j+1})
	= \dt^{-\alpha} \sum_{j = 0}^{n} (-1)^{j} \binom{\alpha}{j} V(x_{i}, t_{n-j+1})
	= \dt^{-\alpha} \sum_{j = 0}^{n} (-1)^{j} \binom{\alpha}{j} V_{i}^{n-j+1}
	= \dt^{-\alpha} (-1)^{0} \binom{\alpha}{0} V_{i}^{n+1} + \dt^{-\alpha} \sum_{j = 1}^{n} (-1)^{j} \binom{\alpha}{j} V_{i}^{n-j+1}
	= \dt^{-\alpha} V_{i}^{n+1} + \dt^{-\alpha} \sum_{j = 1}^{n} (-1)^{j} \binom{\alpha}{j} V_{i}^{n-j+1}
	\end{dmath}
	
	\begin{dmath}
	{}_{t_{1}}D_{t_{n+1}}^{\alpha} V(x_{i},t)
	= \dt^{-\alpha} V_{i}^{n+1} + \dt^{-\alpha} \sum_{j = 1}^{n} (-1)^{j} \binom{\alpha}{j} V_{i}^{n-j+1}
	\end{dmath}

\noindent\rule{\linewidth}{0.4pt}
	\begin{equation}
	\binom{\alpha}{0} = 1, \binom{\alpha}{1} = \alpha, \binom{\alpha}{j+1} = \binom{\alpha}{j}\frac{\alpha - i}{i + 1}
	\end{equation}

\noindent\rule{\linewidth}{0.4pt}
	\begin{dmath}
	Q1(x,t;s) + \dt^{-\alpha} V_{i}^{n+1} + \dt^{-\alpha} \sum_{j = 1}^{n} (-1)^{j} \binom{\alpha}{j} V_{i}^{n-j+1} + [U(x;s) + V(x,t)]\cdot [ Q2(x,t;s) +  Q3(x,t;s) +  {}_{s}J^{1-\alpha}_{t}V_{x}(x,t)]=a \cdot (U_{xxx}(x;s) + V_{xxx}(x,t))
	\end{dmath}
Explicit numerical scheme:
	\begin{dmath}
	Q1(x_{i},t_{n};s) + \dt^{-\alpha} V_{i}^{n+1} + \dt^{-\alpha} \sum_{j = 1}^{n} (-1)^{j} \binom{\alpha}{j} V_{i}^{n-j+1} + [U(x_{i};s) + V_{i}^{n}]\cdot [ Q2(x_{i},t_{n};s) +  Q3(x_{i},t_{n};s) + \frac{1}{2\dx} {}_{t_{1}}J^{1-\alpha}_{t_{n}}\{V^{n}_{i+1} - V^{n}_{i-1}\}]=a \cdot (U_{xxx}(x_{i};s) + V_{xxx}(x_{i},t_{n}))
	\end{dmath}

\noindent\rule{\linewidth}{0.4pt}
	\begin{equation}
	 {}_{s}J^{1-\alpha}_{t}V(x_{i},t) \bigg{|}_{t = t_{n}}
	 =  {}_{t_{1}}J^{1-\alpha}_{t_{n}}V(x_{i},t)
	 = \frac{1}{\Gamma(1-\alpha)} \int_{t_{1}}^{t_{n}} \frac{V(x_{i},\tau)}{(t_{n} - \tau)^{\alpha}} d\tau
	 = \frac{1}{\Gamma(1-\alpha)} \sum_{j = 1}^{n-1} \int_{t_{j}}^{t_{j+1}} \frac{V(x_{i},\tau)}{(t_{n} - \tau)^{\alpha}} d\tau
	\end{equation}
	
	\begin{equation}
	\frac{V(x_{i},\tau) - V_{i}^{j}}{V_{i}^{j+1} - V_{i}^{j}} = \frac{\tau - t_{j}}{\dt},
	V(x_{i},\tau) = V_{i}^{j} + \frac{\tau - t_{j}}{\dt} (V_{i}^{j+1} - V_{i}^{j})
	\end{equation}
	
	\begin{equation}
	 {}_{t_{1}}J^{1-\alpha}_{t_{n}}V(x_{i},t)
	 = \frac{1}{\Gamma(1-\alpha)} \sum_{j = 1}^{n-1} \int_{t_{j}}^{t_{j+1}} \frac{V_{i}^{j} + \frac{\tau - t_{j}}{\dt} (V_{i}^{j+1} - V_{i}^{j})}{(t_{n} - \tau)^{\alpha}} d\tau
	\end{equation}

	\begin{equation}
	 {}_{t_{1}}J^{1-\alpha}_{t_{n}}V(x_{i},t)
	 = \frac{1}{\Gamma(1-\alpha)} \sum_{j = 1}^{n-1} V_{i}^{j} \int_{t_{j}}^{t_{j+1}} \frac{1}{(t_{n} - \tau)^{\alpha}} d\tau
	 + \frac{V_{i}^{j+1} - V_{i}^{j}}{\dt} \int_{t_{j}}^{t_{j+1}} \frac{ \tau - t_{j} }{(t_{n} - \tau)^{\alpha}} d\tau
	\end{equation}
	
	\begin{equation}
	I1(t, j, j+1) = \int_{t_{j}}^{t_{j+1}} \frac{1}{(t - \tau)^{\alpha}} d\tau = \frac{(t - \tau)^{1 - \alpha}}{\alpha - 1} \bigg{|}_{t_{j}}^{t_{j+1}}
	\end{equation}
	
	\begin{equation}
	I2(t, j, j+1) = \int_{t_{j}}^{t_{j+1}} \frac{ \tau - t_{j} }{(t - \tau)^{\alpha}} d\tau = \frac{(t - \tau)^{1 - \alpha}[(\alpha - 1)\tau - (\alpha - 2)t_{j} - t]}{(\alpha - 1)(\alpha - 2)} \bigg{|}_{t_{j}}^{t_{j+1}}
	\end{equation}
	
	\begin{equation}
	 {}_{t_{1}}J^{1-\alpha}_{t_{n}}V(x_{i},t)
	 = \frac{1}{\Gamma(1-\alpha)} \sum_{j = 1}^{n-1} V_{i}^{j} I1(t_{n}, j, j+1)
	 + \frac{V_{i}^{j+1} - V_{i}^{j}}{\dt} I2(t_{n}, j, j+1)
	\end{equation}
	
\noindent\rule{\linewidth}{0.4pt}
	\begin{equation}
	{}_{t_{1}}J^{1-\alpha}_{t_{n+1}}V(x_{i},t)
	 = \frac{1}{\Gamma(1-\alpha)} \int_{t_{1}}^{t_{n+1}} \frac{V(x_{i},\tau)}{(t_{n+1} - \tau)^{\alpha}} d\tau
	 = \frac{1}{\Gamma(1-\alpha)} \sum_{j = 1}^{n} \int_{t_{j}}^{t_{j+1}} \frac{V(x_{i},\tau)}{(t_{n} - \tau)^{\alpha}} d\tau
	\end{equation}
	
	\begin{equation}
	 {}_{t_{1}}J^{1-\alpha}_{t_{n+1}}V(x_{i},t)
	 = \frac{1}{\Gamma(1-\alpha)} \sum_{j = 1}^{n} \int_{t_{j}}^{t_{j+1}} \frac{V_{i}^{j} + \frac{\tau - t_{j}}{\dt} (V_{i}^{j+1} - V_{i}^{j})}{(t_{n+1} - \tau)^{\alpha}} d\tau
	\end{equation}
	
	\begin{equation}
	 {}_{t_{1}}J^{1-\alpha}_{t_{n+1}}V(x_{i},t)
	 = \frac{1}{\Gamma(1-\alpha)} \sum_{j = 1}^{n} V_{i}^{j} \int_{t_{j}}^{t_{j+1}} \frac{1}{(t_{n+1} - \tau)^{\alpha}} d\tau
	 + \frac{V_{i}^{j+1} - V_{i}^{j}}{\dt} \int_{t_{j}}^{t_{j+1}} \frac{ \tau - t_{j} }{(t_{n+1} - \tau)^{\alpha}} d\tau
	\end{equation}

	\begin{equation}
	 {}_{t_{1}}J^{1-\alpha}_{t_{n+1}}V(x_{i},t)
	 = \frac{1}{\Gamma(1-\alpha)} \sum_{j = 1}^{n} V_{i}^{j} I1(t_{n+1}, j, j+1)
	 + \frac{V_{i}^{j+1} - V_{i}^{j}}{\dt} I2(t_{n+1}, j, j+1)
	\end{equation}
	
	\begin{dmath}
	 {}_{t_{1}}J^{1-\alpha}_{t_{n+1}}V(x_{i},t)
	 =\frac{1}{\Gamma(1-\alpha)} \left[ V_{i}^{n} I1(t_{n+1}, n, n+1) + \frac{V_{i}^{n+1} - V_{i}^{n}}{\dt} I2(t_{n+1}, n, n+1) \right] + \frac{1}{\Gamma(1-\alpha)} \sum_{j = 1}^{n-1} V_{i}^{j} I1(t_{n+1}, j, j+1) + \frac{V_{i}^{j+1} - V_{i}^{j}}{\dt} I2(t_{n+1}, j, j+1)
	\end{dmath}
	
	\begin{equation}
	fracIn1(n,i)
	 = \frac{1}{\Gamma(1-\alpha)} \sum_{j = 1}^{n-1} V_{i}^{j} I1(t_{n+1}, j, j+1) + \frac{V_{i}^{j+1} - V_{i}^{j}}{\dt} I2(t_{n+1}, j, j+1)
	\end{equation}

	\begin{equation}
	 {}_{t_{1}}J^{1-\alpha}_{t_{n+1}}V(x_{i},t)
	 =\frac{1}{\Gamma(1-\alpha)} \left[ V_{i}^{n} I1(t_{n+1}, n, n+1) + \frac{V_{i}^{n+1} - V_{i}^{n}}{\dt} I2(t_{n+1}, n, n+1) \right] + fracIn1(n,i)
	\end{equation}

\noindent\rule{\linewidth}{0.4pt}
	\begin{dmath}
	Q1(x_{i},t_{n+1};s) + \dt^{-\alpha} V_{i}^{n+1} + \dt^{-\alpha} \sum_{j = 1}^{n} (-1)^{j} \binom{\alpha}{j} V_{i}^{n-j+1}
	+ \frac{1}{2}[U(x_{i};s) + V_{i}^{n+1}]\cdot [ Q2(x_{i},t_{n};s) +  Q3(x_{i},t_{n};s) + \frac{1}{2\dx} {}_{t_{1}}J^{1-\alpha}_{t_{n}}\{V_{i+1} - V_{i-1}\}]
	+ \frac{1}{2}[U(x_{i};s) + V_{i}^{n}]\cdot [ Q2(x_{i},t_{n+1};s) +  Q3(x_{i},t_{n+1};s) + \frac{1}{2\dx} {}_{t_{1}}J^{1-\alpha}_{t_{n+1}}\{V_{i+1} - V_{i-1}\}]=a \cdot (U_{xxx}(x_{i};s) + V_{xxx}(x_{i},t_{n+1}))
	\end{dmath}
	
	\begin{equation}
	D1(n,i) = \dt^{-\alpha} \sum_{j = 1}^{n} (-1)^{j} \binom{\alpha}{j} V_{i}^{n-j+1}
	\end{equation}
\noindent\rule{\linewidth}{0.4pt}
Implicit numerical scheme:
	\begin{dmath}
	Q1(x_{i},t_{n+1};s) + \dt^{-\alpha} V_{i}^{n+1} + D1(n,i)
	+ \frac{1}{2}[U(x_{i};s) + V_{i}^{n+1}]\cdot [ Q2(x_{i},t_{n};s) +  Q3(x_{i},t_{n};s) + \frac{1}{2\dx} {}_{t_{1}}J^{1-\alpha}_{t_{n}}\{V_{i+1} - V_{i-1}\}]
	+ \frac{1}{2}[U(x_{i};s) + V_{i}^{n}]\cdot [ Q2(x_{i},t_{n+1};s) +  Q3(x_{i},t_{n+1};s) + \frac{1}{2\dx} {}_{t_{1}}J^{1-\alpha}_{t_{n+1}}\{V_{i+1} - V_{i-1}\}]=a \cdot (U_{xxx}(x_{i};s) + V_{xxx}(x_{i},t_{n+1}))
	\end{dmath}

\noindent\rule{\linewidth}{0.4pt}
	Explicit numerical scheme:
	\begin{dmath}
	Q1(x_{i},t_{n};s) + \dt^{-\alpha} V_{i}^{n+1} + D1(n,i) + [U(x_{i};s) + V_{i}^{n}]\cdot [ Q2(x_{i},t_{n};s) +  Q3(x_{i},t_{n};s) + \frac{1}{2\dx} {}_{t_{1}}J^{1-\alpha}_{t_{n}}\{V^{n}_{i+1} - V^{n}_{i-1}\}]=a \cdot (U_{xxx}(x_{i};s) + V_{xxx}(x_{i},t_{n}))
	\end{dmath}
	
	\begin{equation}
	V_{xxx}(x_{i},t_{n}) = {V_{i}^{n}}_{xxx} = \frac{V_{i+2}^{n} - 2{V}_{i+1}^{n} + 2 {V}_{i-1}^{n} - V_{i-2}^{n}}{\dx^{3}}
	\end{equation}

	\begin{dmath}
	\dt^{-\alpha} V_{i}^{n+1} = - Q1(x_{i},t_{n};s) - D1(n,i) - [U(x_{i};s) + V_{i}^{n}]\cdot [ Q2(x_{i},t_{n};s) +  Q3(x_{i},t_{n};s) + \frac{1}{2\dx} {}_{t_{1}}J^{1-\alpha}_{t_{n}}\{V^{n}_{i+1} - V^{n}_{i-1}\}] + a \cdot (U_{xxx}(x_{i};s) + V_{xxx}(x_{i},t_{n}))
	\end{dmath}

\end{document}
